\documentclass[12pt]{article}
\usepackage{ucs}
\usepackage[utf8x]{inputenc}
\usepackage[english,russian]{babel}
\pagestyle{empty}
\usepackage{amsmath}

\begin{document}
  $$x^{x^{ln\left(x\right)}}$$
После упрощения получаем
    $$x^{x^{ln\left(x\right)}}$$
По правилу такой дичи, как $f ^ {g}$: $\left(f ^ {g}\right)' = (e ^ {ln\left(f\right) * g})' = e ^ {ln\left(f\right) * g} * \left(ln\left(f\right) * g\right)'$, где $\alpha = x$, а $f = x^{ln\left(x\right)}$\\
Продифференцируем $f = ln\left(x\right)$:\\По правилу производной логарифма $\left(ln\left(f\right)\right)' = \frac{f'}{f}$, где $f = x$\\
Продифференцируем $f = x$:\\$x$ - главная переменная\\$\left(x\right)' = 1$\\$\left(ln\left(x\right)\right)' = \frac{1}{x}$\\
Теперь продифференцируем $g = x^{ln\left(x\right)}$:\\По правилу такой дичи, как $f ^ {g}$: $\left(f ^ {g}\right)' = (e ^ {ln\left(f\right) * g})' = e ^ {ln\left(f\right) * g} * \left(ln\left(f\right) * g\right)'$, где $\alpha = x$, а $f = ln\left(x\right)$\\
Продифференцируем $f = ln\left(x\right)$:\\По правилу производной логарифма $\left(ln\left(f\right)\right)' = \frac{f'}{f}$, где $f = x$\\
Продифференцируем $f = x$:\\$x$ - главная переменная\\$\left(x\right)' = 1$\\$\left(ln\left(x\right)\right)' = \frac{1}{x}$\\
Теперь продифференцируем $g = ln\left(x\right)$:\\По правилу производной логарифма $\left(ln\left(f\right)\right)' = \frac{f'}{f}$, где $f = x$\\
Продифференцируем $f = x$:\\$x$ - главная переменная\\$\left(x\right)' = 1$\\$\left(ln\left(x\right)\right)' = \frac{1}{x}$\\$\left(x^{ln\left(x\right)}\right)' = e^{ln\left(x\right) \cdot ln\left(x\right)} \cdot \left(\frac{1}{x} \cdot ln\left(x\right) + ln\left(x\right) \cdot \frac{1}{x}\right)$\\Итак, производная равна
    $$e^{x^{ln\left(x\right)} \cdot ln\left(x\right)} \cdot \left(e^{ln\left(x\right) \cdot ln\left(x\right)} \cdot \left(\frac{1}{x} \cdot ln\left(x\right) + ln\left(x\right) \cdot \frac{1}{x}\right) \cdot ln\left(x\right) + x^{ln\left(x\right)} \cdot \frac{1}{x}\right)$$
После упрощения получаем
    $$e^{x^{ln\left(x\right)} \cdot ln\left(x\right)} \cdot \left(e^{ln\left(x\right) \cdot ln\left(x\right)} \cdot \left(\frac{1}{x} \cdot ln\left(x\right) + ln\left(x\right) \cdot \frac{1}{x}\right) \cdot ln\left(x\right) + x^{ln\left(x\right)} \cdot \frac{1}{x}\right)$$
\end{document}